Start on theorem about high-level language Continue running low-level program after recovery

src/Fs9.v
@@ -111,6 +111,52 @@ Eval simpl in texec (TWrite 0 1 ;; (v <- (TRead 0) ; (TWrite 1 v) ;; THalt)) (TS
 Eval simpl in texec (TBegin ;; TWrite 0 1 ;; TWrite 1 1 ;; TEnd ;; THalt) (TSt st_init None).
 Eval simpl in texec (TBegin ;; TWrite 0 1 ;; TWrite 1 1 ;; THalt) (TSt st_init None).
 
+Fixpoint find_last_committed_write (p:tprog) (s:tstate) (bw:block) (vu:nat) (vc:nat) :=
+  let (d, ad) := s in
+  match p with
+  | THalt => vc
+  | TRead b rx => find_last_committed_write (rx (TRValue (st_read d b))) (TSt d ad) bw vu vc
+  | TWrite b v rx =>
+    match ad with
+      | None   => find_last_committed_write (rx TRSucc) (TSt (st_write d b v) ad) bw v v
+      | Some x => find_last_committed_write (rx TRSucc) (TSt d (Some (st_write x b v))) bw (if eq_nat_dec bw b then v else vu) vc 
+    end
+  | TBegin rx => 
+    match ad with
+    | None   => find_last_committed_write (rx TRSucc) (TSt d (Some d)) bw vu vc
+    | Some _ => find_last_committed_write (rx TRFail) (TSt d ad) bw vu vc
+    end
+  | TEnd rx =>
+    match ad with
+    | Some d => find_last_committed_write (rx TRSucc) (TSt d None) bw vc vc
+    | None   => find_last_committed_write (rx TRFail) (TSt d ad) bw vu vc
+    end
+  end.
+
+Theorem trans_committed_last_write:
+  forall s prog b,
+    texec prog (TSt st_init None) = s ->
+    find_last_committed_write prog s b 0 0 = st_read s.(TSDisk) b.
+Proof.
+  intro.
+  induction prog.
+  intuition.
+  (* read *)
+  - intros.
+    admit.
+  (* write *)
+  - intros.
+    admit.
+  (* begin *)
+  - intros.
+    admit.
+  (* end *)
+  - intros.
+    admit.
+  (* halt *)
+  - intros.
+Admitted.
+
 Close Scope tprog_scope.
 
 
@@ -251,12 +297,10 @@ Inductive pstep : pstate -> pprog -> pstate -> Prop :=
   | PsGetTx: forall d l c rx s,
     pstep (PSt d l c) (rx c) s ->
     pstep (PSt d l c) (PGetTx rx) s
-  | PsCrash: forall p s,
-    pstep s p (pexec (do_trecover PHalt) s)
-    (* XXX: how to continue running after recovery ? *)
-  .
-
-
+  | PsCrash: forall p d l c l' c',
+    (* XXX need some theorem about recovery *)
+    pstep (PSt d l c) p (PSt (PSDisk (pexec (do_trecover p) (PSt d l c))) l' c')
+    (* XXX: how to continue running after recovery ? *).
 
 Fixpoint log_flush (p:list (block*value)) (d:storage) : storage :=
   match p with
